theories/uni-binv.v
@@ -1,0 +1,180 @@
+Require Import
+  HoTT.Basics
+  HoTT.Types
+  HoTT.Tactics.
+
+Definition IsBinv {A B} (f : A -> B) :=
+  {_ : {g : B -> A | g o f == idmap}
+     | {h : B -> A | f o h == idmap} }.
+
+Definition linv_isbinv {A B : Type} {f : A -> B} (S : IsBinv f)
+  : B -> A
+  := S.1.1.
+
+Definition rinv_isbinv {A B : Type} {f : A -> B} (S : IsBinv f)
+  : B -> A
+  := S.2.1.
+
+Definition lhomot_isbinv {A B : Type} {f : A -> B} (S : IsBinv f)
+  : linv_isbinv S o f == idmap
+  := S.1.2.
+
+Lemma lpath_isbinv `{Funext} {A B : Type} {f : A -> B} (S : IsBinv f)
+  : linv_isbinv S o f = idmap.
+Proof.
+  funext a. apply lhomot_isbinv.
+Defined.
+
+Definition rhomot_isbinv {A B : Type} {f : A -> B} (S : IsBinv f)
+  : f o rinv_isbinv S == idmap
+  := S.2.2.
+
+Lemma rpath_isbinv `{Funext} {A B : Type} {f : A -> B} (S : IsBinv f)
+  : f o rinv_isbinv S = idmap.
+Proof.
+  funext a. apply rhomot_isbinv.
+Defined.
+
+Lemma homot_rinv_isbinv {A B : Type} {f : A -> B} (S T : IsBinv f)
+  : rinv_isbinv S == rinv_isbinv T.
+Proof.
+  intro b.
+  refine ((lhomot_isbinv S (rinv_isbinv S b))^ @ _).
+  refine (ap (linv_isbinv S) (rhomot_isbinv S b) @ _).
+  refine (ap (linv_isbinv S) (rhomot_isbinv T b)^ @ _).
+  exact ((lhomot_isbinv S (rinv_isbinv T b))).
+Defined.
+
+Lemma path_rinv_isbinv `{Funext} {A B : Type} {f : A -> B} (S T : IsBinv f)
+  : rinv_isbinv S = rinv_isbinv T.
+Proof.
+  funext b. apply homot_rinv_isbinv.
+Defined.
+
+Lemma homot_linv_isbinv {A B : Type} {f : A -> B} (S T : IsBinv f)
+  : linv_isbinv S == linv_isbinv T.
+Proof.
+  intro b.
+  refine (ap (linv_isbinv S) (rhomot_isbinv S b)^ @ _).
+  refine (lhomot_isbinv S (rinv_isbinv S b) @ _).
+  refine ((lhomot_isbinv T (rinv_isbinv S b))^ @ _).
+  exact (ap (linv_isbinv T) (rhomot_isbinv S b)).
+Defined.
+
+Lemma path_linv_isbinv `{Funext} {A B : Type} {f : A -> B} (S T : IsBinv f)
+  : linv_isbinv S = linv_isbinv T.
+Proof.
+  funext b. apply homot_linv_isbinv.
+Defined.
+
+Lemma homot_linv_rinv_isbinv {A B : Type} {f : A -> B} (S : IsBinv f)
+  : linv_isbinv S == rinv_isbinv S.
+Proof.
+  intro b.
+  exact (ap (linv_isbinv S) (rhomot_isbinv S b)^
+         @ lhomot_isbinv S (rinv_isbinv S b)).
+Defined.
+
+Lemma path_linv_rinv_isbinv `{Funext} {A B : Type} {f : A -> B} (S : IsBinv f)
+  : linv_isbinv S = rinv_isbinv S.
+Proof.
+  funext b. apply homot_linv_rinv_isbinv.
+Defined.
+
+Lemma ap_composef {A B C D : Type} (g : C -> D) (F : (A -> B) -> C)
+  {f1 f2} (h : f1 = f2) :
+  ap (fun f : A -> B => g (F f)) h =
+  ap g (ap (fun f : A -> B => F f) h).
+Proof.
+  by path_induction.
+Defined.
+
+Lemma hprop_isbinv `{Funext} {A B} (f : A -> B) : IsHProp (IsBinv f).
+Proof.
+  apply hprop_allpath.
+  intros [[g P1] [h1 R1]] [[g2 P2] [h2 R2]].
+  set (p := path_linv_isbinv ((g; P1); (h1; R1)) ((g2; P2); (h2; R2))).
+  cbn in p; induction p.
+  set (p := path_rinv_isbinv ((g; P1); (h1; R1)) ((g; P2); (h2; R2))).
+  cbn in p; induction p.
+  set (p := path_linv_rinv_isbinv ((g; P1); (h1; R1))).
+  cbn in p; induction p.
+  pose proof (h1 := (rpath_isbinv ((g; P1); (g; R1)))^).
+  pose proof (h2 := (lpath_isbinv ((g; P1); (g; R1)))^).
+  srapply path_sigma; cbn in*.
+  - srapply path_sigma; cbn in *.
+    + funext b.
+      exact ((ap (fun i => i (g b)) h2)
+              @ P1 (g b) @ (P2 (g b))^
+              @ (ap (fun i => i (g b)) h2^)).
+    + cbn in *.
+      funext b.
+      rewrite transport_forall_constant.
+      transport_path_forall_hammer.
+      rewrite transport_paths_Fl.
+      hott_simpl.
+      generalize dependent P2.
+      generalize dependent P1.
+      refine (
+        paths_ind
+          _
+          (fun F R =>
+forall P1 P2 : F == idmap,
+(((ap (fun i : A -> A => i (F b)) R @ P1 (F b)) @ (P2 (F b))^) @
+ ap (fun i : A -> A => i (F b)) R^)^ @ P1 b = 
+P2 b
+          )
+          _
+          _
+          h2
+      ).
+      intros.
+      hott_simpl.
+      rewrite inv_pp.
+      rewrite inv_V.
+      hott_simpl.
+  - rewrite transport_const.
+    srapply path_sigma; cbn in *.
+    + funext b.
+      exact ((ap (fun i => g (i b)) h1)
+              @ ap g (R1 b) @ ap g (R2 b)^
+              @ (ap (fun i => g (i b)) h1^)).
+    + cbn in *.
+      funext b.
+      rewrite transport_forall_constant.
+      transport_path_forall_hammer.
+      rewrite transport_paths_Fl.
+      rewrite <- ap_V.
+      rewrite inv_pp.
+      rewrite inv_pp.
+      rewrite inv_pp.
+      rewrite ap_V.
+      hott_simpl.
+      rewrite ap_pp.
+      rewrite ap_pp.
+      rewrite ap_pp.
+      rewrite <- ap_compose.
+      rewrite <- ap_compose.
+      rewrite <- (ap_composef f (fun i : B -> B => g (i b)) h1).
+      rewrite ap_V.
+      rewrite ap_V.
+      rewrite <- (ap_composef f (fun i : B -> B => g (i b)) h1).
+      generalize dependent R2.
+      generalize dependent R1.
+      refine (
+        paths_ind _
+          (fun F R =>
+forall rtg stg : F == idmap,
+(((ap (fun f0 : B -> B => F (f0 b)) R @
+   ap F (stg b)) @
+  (ap F (rtg b))^) @
+ (ap (fun f0 : B -> B => F (f0 b)) R)^) @ rtg b = 
+stg b
+          )
+          _
+          _
+          h1
+      ).
+      intros.
+      hott_simpl.
+Defined.
